verified lock-free counter

fairness/lawyer/examples/lf_counter/lf_counter.v
@@ -55,10 +55,22 @@ Section WaitMap.
     - apply alloc_local_update; eauto. done.
   Qed.  
 
+  Lemma wm_get0 wm i
+    (DOM: i ∈ dom wm):
+    wm_auth wm ==∗ wm_auth wm ∗ val_toks i 0.
+  Proof using.
+    iIntros "WM". rewrite -own_op. rewrite /wm_auth.
+    iApply (own_update with "[$]"). apply auth_update_alloc.
+    apply elem_of_dom in DOM as [? ITH]. 
+    etrans. 
+    - eapply insert_alloc_local_update; eauto. reflexivity.
+    - rewrite insert_id; [| done]. reflexivity. 
+  Qed.
+
 End WaitMap.
 
 
-Section Nondet.
+Section LFCounter.
   Context `{ODd: OfeDiscrete DegO} `{ODl: OfeDiscrete LevelO}.
   Context `{LEl: @LeibnizEquiv (ofe_car LevelO) (ofe_equiv LevelO)}.
   
@@ -99,22 +111,64 @@ Section Nondet.
     intros [??]. simpl. rewrite /gt. solve_decision.
   Qed.
 
-  Definition wm_interp `{LFCG Σ} π0 c (wm: gmap nat nat): iProp Σ :=
+  Definition wm_waits `{LFCG Σ} π__cnt c (wm: gmap nat nat): iProp Σ :=
     [∗ map] i ↦ n ∈ filter (gt c ∘ fst) wm, 
-      (∃ r, cp π0 d0 ∨ val_toks i (n - r)).
+      (∃ r, cp_mul π__cnt d0 (r * INCR_ITER_LEN) ∗ val_toks i (n - r) ∗ ⌜ r <= n ⌝).
+
+  Definition set_max (X: gset nat): nat :=
+    list_max $ elements $ X.
+
+  Lemma set_max_spec X n:
+    set_max X ≤ n ↔ set_Forall (λ k, k ≤ n) X.
+  Proof using.
+    rewrite /set_max. rewrite list_max_le.
+    by rewrite set_Forall_elements.
+  Qed.
+
+  (* TODO: move, does it exist already? *)
+  Lemma list_max_elems X:
+    forall x, x ∈ X -> x <= list_max X.
+  Proof using.
+    clear. 
+    induction X.
+    { set_solver. }
+    intros x. rewrite elem_of_cons. intros [->|?]; simpl. 
+    - lia.
+    - etrans; [| apply Nat.le_max_r]. eauto.
+  Qed.
+
+  Lemma set_max_elems X:
+    forall x, x ∈ X -> x <= set_max X.
+  Proof using.
+    intros x IN. rewrite /set_max.
+    apply list_max_elems. by apply elem_of_elements.
+  Qed.
 
   Definition wm_eb (wm: gmap nat nat): iProp Σ :=
-    exc_lb $ list_max $ elements $ (map_img wm: gset nat). 
+    exc_lb (set_max (map_img wm: gset nat) * INCR_ITER_LEN). 
 
-  Definition cnt_inv_inner `{LFCG Σ} (cnt: loc) (π0: Phase): iProp Σ :=
-    ∃ (c: nat) wm, cnt ↦ #c ∗ wm_auth wm ∗ wm_interp π0 c wm ∗ wm_eb wm. 
+  Definition wm_interp `{LFCG Σ} π__cnt c: iProp Σ :=
+    ∃ wm, wm_auth wm ∗ wm_waits π__cnt c wm ∗ wm_eb wm ∗ ⌜ dom wm = set_seq 0 (S c) ⌝.
+
+  Definition cnt_inv_inner `{LFCG Σ} (cnt: loc) (π__cnt: Phase): iProp Σ :=
+    ∃ (c: nat), cnt ↦ #c ∗ wm_interp π__cnt c. 
 
   Definition cnt_ns := nroot.@"cnt".
-  Definition cnt_inv `{LFCG Σ} cnt π0 := inv cnt_ns (cnt_inv_inner cnt π0).
+  Definition cnt_inv `{LFCG Σ} cnt π__cnt := inv cnt_ns (cnt_inv_inner cnt π__cnt).
 
   Context {OBLS_AMU: @AMU_lift_MU _ _ _ oGS' _ EM _ (↑ nroot)}.
   Context {OBLS_AMU__f: forall τ, @AMU_lift_MU__f _ _ _ τ oGS' _ EM _ ⊤}.
   Context {NO_OBS_POST: ∀ τ v, obls τ ∅ -∗ fork_post τ v}.
+
+  (* TODO: move *)
+  Global Instance cp_mul_Timeless π d n: Timeless (cp_mul π d n).
+  Proof using.
+    rewrite obligations_resources.cp_mul_unseal.
+    rewrite /obligations_resources.cp_mul_def.
+    clear.
+    apply big_sepL_timeless_id.
+    induction n; apply _.
+  Qed.
 
   Definition incr_impl: val :=
     rec: "incr_impl" "c" :=
@@ -124,16 +178,187 @@ Section Nondet.
   . 
 
   Definition incr: val :=
-    λ: "c", incr_impl "c". 
+    λ: "c", incr_impl "c".
 
-  Lemma incr_impl_spec `{LFCG Σ} τ π cnt π0
-    (PH: phase_le π0 π):
-    {{{ cnt_inv cnt π0 ∗ exc_lb (S INCR_ITER_LEN) ∗ 
-        cp π0 d1 ∗ cp_mul π d0 INCR_ITER_LEN ∗ 
+  (* TODO: move *)
+  Global Instance frame_BOU p E n R P Q:
+    (Frame p R P Q) →
+    Frame p R (BOU E n P) (BOU E n Q).
+  Proof using.
+    red. intros FRAME. iIntros "[R BOU]".
+    red in FRAME.
+    iMod "BOU" as "?". iModIntro.
+    iApply FRAME. iFrame.
+  Qed.
+
+  (* TODO: move *)
+  Global Instance FromExist_BOU {A: Type} E n P (Φ: A -> iProp Σ):
+    FromExist P Φ ->
+    FromExist (BOU E n P) (fun x => BOU E n (Φ x)).
+  Proof using.
+    rewrite /FromExist. iIntros (EX) "[%x BOU]".
+    iMod "BOU". iModIntro.
+    iApply EX. by iExists _.
+  Qed.
+
+  Lemma eb_wm_incr wm c:
+    wm_eb wm -∗ BOU ∅ INCR_ITER_LEN
+      (wm_eb (<[c:=(default 0 (wm !! c) + 1)]> wm)).
+  Proof using.
+    clear INCR_LS_LB. 
+    iIntros "EB".
+    iApply OU_BOU_rep. iApply (OU_rep_wand with "[]").
+    2: { iApply increase_eb_upd_rep. iFrame. }
+
+    iApply exc_lb_le.
+    rewrite -Nat.mul_succ_l. apply PeanoNat.Nat.mul_le_mono_r. 
+    apply set_max_spec. rewrite /set_Forall. intros i.
+    rewrite elem_of_map_img. setoid_rewrite lookup_insert_Some.
+    rewrite -(Nat.add_1_r (set_max _)).
+    intros [n [[<- <-] | [? ITH]]].
+    - destruct (wm !! c) eqn:CTH; simpl; [| lia].
+      apply Plus.plus_le_compat_r_stt.
+      apply set_max_elems. eapply elem_of_map_img; eauto.
+    - etrans; [apply set_max_elems| ].
+      { eapply @elem_of_map_img.
+        3: eexists; eauto.
+        all: apply _. }
+      lia.
+  Qed.
+    
+  Lemma wm_alloc_tok `{LFCG Σ} π__cnt c:
+    wm_interp π__cnt c -∗ BOU ∅ INCR_ITER_LEN (wm_interp π__cnt c ∗ val_tok c).
+  Proof using.
+    clear INCR_LS_LB.
+    iIntros "(%wm & AUTH & WAITS & #EB & %DOM)".
+    iMod (wm_alloc _ c with "[$]") as "[AUTH TOK]".
+    iFrame "TOK". 
+    rewrite /wm_interp.
+    iExists _. iFrame "AUTH".
+
+    iApply (BOU_frame_l with "[WAITS]").
+    { rewrite /wm_waits.
+      rewrite map_filter_insert_not; [done| ].
+      simpl. lia. }
+
+    iApply BOU_frame_r.
+    { iPureIntro. rewrite dom_insert_L. rewrite <- DOM.
+      apply subseteq_union_1_L. apply singleton_subseteq_l.
+      rewrite DOM. apply elem_of_set_seq. lia. }
+
+    by iApply eb_wm_incr. 
+  Qed.
+
+  Lemma wm_incr `{LFCG Σ} π__cnt c:
+    wm_interp π__cnt c -∗ cp π__cnt d1 -∗ BOU ∅ (INCR_ITER_LEN + 1) (wm_interp π__cnt (S c)).
+  Proof using DEG01. 
+    clear ODl ODd OBLS_AMU__f OBLS_AMU NO_OBS_POST LEl INCR_LS_LB. 
+    iIntros "(%wm & AUTH & WAITS & #EB & %DOM) CP1".
+    iMod (wm_alloc _ (S c) with "[$]") as "[AUTH TOK]".
+    iMod (wm_get0 _ c with "[$]") as "[AUTH TOKS0]".
+    { rewrite dom_insert_L. rewrite DOM.
+      apply elem_of_union. right. apply elem_of_set_seq. lia. }    
+    rewrite /wm_interp. iExists _. iFrame "AUTH".
+
+    rewrite bi.sep_assoc. iApply BOU_frame_r.
+    { iPureIntro. rewrite dom_insert_L. rewrite DOM.
+      rewrite (set_seq_S_end_union_L _ (S c)). done. }
+
+    iMod (eb_wm_incr with "[$]") as "#EB'"; [lia| ]. 
+    iApply BOU_frame_r; [iApply "EB'"| ]. 
+    
+    rewrite not_elem_of_dom_1.
+    2: { rewrite DOM. intros ?%elem_of_set_seq. lia. }
+    simpl.
+
+    assert (c ∈ dom wm) as [k CTH]%elem_of_dom.
+    { rewrite DOM. apply elem_of_set_seq. lia. }
+
+    rewrite /wm_waits.
+    rewrite map_filter_insert_not.
+    2: { intros. simpl. lia. }
+
+    rewrite {3 4}(map_split wm c). rewrite CTH. simpl.  
+    rewrite !map_filter_union.
+    2, 3: apply map_disjoint_dom; set_solver. 
+    rewrite !big_sepM_union.
+    2, 3: apply map_disjoint_dom; eapply disjoint_subseteq;
+          [apply _| apply dom_filter_subseteq | apply dom_filter_subseteq| ];
+          set_solver. 
+    iDestruct "WAITS" as "[_ WAITS']". iApply (BOU_frame_r with "[WAITS']").
+    { iApply (big_opM_proper_2 with "[$]").
+      2: { intros ????? EQ.
+           erewrite leibniz_equiv_iff in EQ. by subst. }
+      apply map_equiv_iff. intros i.
+      rewrite !map_filter_lookup.
+      destruct (delete c wm !! i) eqn:ITH.
+      2: { done. }
+      simpl. apply lookup_delete_Some in ITH as [? ITH].
+      rewrite !option_guard_decide.
+      apply mk_is_Some, elem_of_dom in ITH. rewrite DOM in ITH.
+      apply elem_of_set_seq in ITH. 
+      apply leibniz_equiv_iff. destruct decide, decide; try lia. done. }
+
+    rewrite map_filter_singleton. simpl. destruct decide; [| lia].
+    rewrite big_sepM_singleton.
+    iExists k. rewrite Nat.sub_diag. iFrame "TOKS0".
+    iMod (exchange_cp_upd with "[$] []").
+    4: { iModIntro. iFrame. iPureIntro. lia. }
+    { reflexivity. }
+    { apply DEG01. }
+    iApply (exc_lb_le with "EB").
+    apply Nat.mul_le_mono_r. 
+    apply set_max_elems. eapply elem_of_map_img; eauto.
+  Qed. 
+
+  Lemma wmi_swap `{LFCG Σ} c c' π__cnt
+    (NEQ: c ≠ c'):
+    wm_interp π__cnt c' -∗ val_tok c -∗ wm_interp π__cnt c' ∗ cp_mul π__cnt d0 INCR_ITER_LEN.
+  Proof using.
+    clear DEG01 ODl ODd OBLS_AMU__f OBLS_AMU NO_OBS_POST LEl INCR_LS_LB. 
+    iIntros "(%wm & AUTH & WAITS & #EB & %DOM) TOK".
+    rewrite /wm_interp.
+    iApply bi.sep_exist_r. iExists _. iFrame "EB". iClear "EB".
+    rewrite bi.sep_comm !bi.sep_assoc. iSplitL; [| done].  
+    rewrite /wm_waits.
+    iDestruct (wm_auth_toks_ge with "[$] [$]") as %LT.
+    destruct LT as (K & CTH & _).
+    assert (c < c') as LT. 
+    { apply mk_is_Some, elem_of_dom in CTH. rewrite DOM in CTH.
+      apply elem_of_set_seq in CTH. lia. }
+    rewrite (map_split wm c). rewrite CTH. simpl.
+    rewrite !map_filter_union.
+    2: apply map_disjoint_dom; set_solver. 
+    rewrite !big_sepM_union.
+    2: apply map_disjoint_dom; eapply disjoint_subseteq;
+          [apply _| apply dom_filter_subseteq | apply dom_filter_subseteq| ];
+          set_solver.
+    iDestruct "WAITS" as "[C WAITS']". iFrame "WAITS'".
+    rewrite map_filter_singleton. simpl. destruct decide; [| lia].
+    rewrite big_opM_singleton. iDestruct "C" as "(%r & CPS & TOKS & %LErk)".
+    iCombine "TOK TOKS" as "TOKS".
+    iDestruct (wm_auth_toks_ge with "[$] [$]") as %BOUNDc. iFrame "AUTH".
+    destruct BOUNDc as (?&CTH_&BOUNDc).
+    erewrite lookup_union_Some_l in CTH_; [| apply lookup_singleton].
+    inversion CTH_. subst x.
+    destruct r. 
+    { lia. }
+    rewrite Nat.mul_succ_l. iDestruct (cp_mul_split with "CPS") as "[? CPS]".
+    iFrame "CPS".
+    iExists _. iFrame.
+    replace (1 + (K - S r)) with (K - r) by lia. iFrame.
+    iPureIntro. lia.
+  Qed.
+
+  Lemma incr_impl_spec `{LFCG Σ} τ π cnt π__cnt
+    (PH: phase_le π__cnt π):
+    {{{ cnt_inv cnt π__cnt ∗ exc_lb (S INCR_ITER_LEN) ∗ 
+        cp π__cnt d1 ∗ cp_mul π d0 INCR_ITER_LEN ∗ 
         th_phase_frag τ π 1 }}}
       incr_impl #cnt @τ
     {{{ v, RET v; ⌜ True ⌝ }}}.
-  Proof using.
+  Proof using OBLS_AMU INCR_LS_LB DEG01.
+    clear ODl ODd OBLS_AMU__f NO_OBS_POST LEl.     
     iIntros (Φ) "(#INV & #EB & CP1 & CPS & PH) POST".
     iLöb as "IH".
     rewrite /incr_impl.
@@ -143,17 +368,63 @@ Section Nondet.
     wp_bind (! _)%E.
     iApply wp_atomic.
     iInv "INV" as "inv" "CLOS". iModIntro.
-    rewrite {1}/cnt_inv_inner. iDestruct "inv" as ">(%c & %wm & CNT & AUTH & WMI & WMEB)".
+    rewrite {1}/cnt_inv_inner. iDestruct "inv" as ">(%c & CNT & WMI)".
     iApply sswp_MU_wp; [done| ]. iApply (wp_load with "[$]"). iIntros "!> CNT".
- 
+    MU_by_BOU.
+    iApply BOU_weaken; [reflexivity| apply empty_subseteq| iIntros "X"; iApply "X"| ].
+    iMod (wm_alloc_tok with "[$]") as "[WMI TOK]".
+    { lia. }
+    BOU_burn_cp. iApply wp_value.
+    iMod ("CLOS" with "[CNT WMI]") as "_".
+    { iExists _. iFrame. }
+    iModIntro.
 
-  Admitted. 
+    wp_bind (Rec _ _ _)%E. pure_steps.
+
+    wp_bind (_ + _)%E. pure_steps.
+
+    wp_bind (CmpXchg _ _ _)%E.  
+    iApply wp_atomic.
+    iInv "INV" as "inv" "CLOS". iModIntro.
+    rewrite {1}/cnt_inv_inner. iDestruct "inv" as ">(%c' & CNT & WMI)".
+    iApply sswp_MU_wp; [done| ].
+
+    destruct (decide (c' = c)) as [-> | NEQ].
+    - iApply (wp_cmpxchg_suc with "[$]").
+      { done. }
+      { by constructor. }
+      iIntros "!> CNT".
+      MU_by_BOU.
+      iApply BOU_weaken; [reflexivity| apply empty_subseteq| iIntros "X"; iApply "X"| ].
+      iMod (wm_incr with "[$] [$]") as "WMI".
+      { lia. }
+      BOU_burn_cp. iApply wp_value.
+      iMod ("CLOS" with "[CNT WMI]") as "_".
+      { iExists _. replace (Z.of_nat (S c)) with (Z.of_nat c + 1)%Z by lia.
+        iFrame. }
+      iModIntro.
+
+      wp_bind (Snd _)%E. pure_steps. by iApply "POST".
+    - iApply (wp_cmpxchg_fail with "[$]").
+      { set_solver. }
+      { by constructor. }
+      iIntros "!> CNT".
+      iDestruct (wmi_swap with "WMI [$]") as "[WMI CPS']"; [done| ].
+      MU_by_burn_cp. iApply wp_value.  
+      iMod ("CLOS" with "[CNT WMI]") as "_".
+      { iExists _. iFrame. }
+      iModIntro.
+
+      wp_bind (Snd _)%E. do 3 pure_step_cases.
+      iDestruct (cp_mul_weaken with "CPS'") as "CPS'"; [apply PH | reflexivity| ].
+      iApply ("IH" with "[$] [$] [$] [$]"). 
+  Qed.
 
   
-  Lemma incr_spec `{LFCG Σ} τ π cnt π0
-    (PH: phase_le π0 π):
-    {{{ th_phase_eq τ π ∗ cp_mul π0 d1 2 ∗
-        cnt_inv cnt π0 }}}
+  Lemma incr_spec `{LFCG Σ} τ π cnt π__cnt
+    (PH: phase_le π__cnt π):
+    {{{ th_phase_eq τ π ∗ cp_mul π__cnt d1 2 ∗
+        cnt_inv cnt π__cnt }}}
       incr #cnt @ τ
     {{{ v, RET v; ⌜ True ⌝ }}}.
   Proof using OBLS_AMU INCR_LS_LB DEG01.
@@ -171,6 +442,47 @@ Section Nondet.
     { apply PH. }
     { iFrame "#∗". }
     done.
+  Qed.
+
+  (* TODO: move *)
+  Lemma set_max_singleton x:
+    set_max {[ x ]} = x.
+  Proof using.
+    clear.
+    rewrite /set_max. rewrite elements_singleton. simpl. lia.
   Qed. 
-    
-    
+
+  Lemma wmi_init `{LFCPreG Σ} π__cnt:
+    ⊢ BOU ∅ 0 (∃ (L: LFCG Σ), wm_interp π__cnt 0).
+  Proof using.
+    clear -H. 
+    rewrite /wm_interp. iStartProof.
+    iMod (own_alloc (● {[ 0 := 0 ]} ⋅ ◯ _: (authUR (gmapUR nat natUR)))) as (γ) "[AUTH FRAG]".
+    { apply auth_both_valid_2; [| reflexivity].
+      by apply singleton_valid. }
+    set (L := {| γ__wm := γ; |}).
+    iApply OU_BOU_rep.
+    iApply (OU_rep_wand with "[-]").
+    2: { iApply increase_eb_upd_rep0. }
+    iIntros "#EB". 
+    iExists L, _. iFrame. iSplitL.
+    { rewrite /wm_waits. rewrite map_filter_singleton. simpl.
+      destruct decide; [lia| ]. set_solver. }
+    iSplit.
+    - rewrite /wm_eb. simpl. rewrite map_img_singleton_L.
+      by rewrite set_max_singleton.
+    - iPureIntro. rewrite dom_singleton_L. set_solver.
+  Qed.
+
+  Lemma alloc_cnt `{LFCPreG Σ} cnt π__cnt:
+    cnt ↦ #0 -∗ BOU ∅ 0 (∃ (L: LFCG Σ), cnt_inv cnt π__cnt).
+  Proof using.
+    iIntros "CNT".
+    iMod wmi_init as "(%L & WMI)".
+    iMod (inv_alloc cnt_ns _ (cnt_inv_inner cnt π__cnt) with "[-]") as "#?".
+    { iExists _. iNext. iFrame. }
+    iModIntro. iExists _. iFrame "#∗".
+  Qed.
+
+End LFCounter.
+  
